alpha_equiv complete

qcp/ast/annotated_C/alpha_equiv.c
@@ -5,9 +5,8 @@ bool alpha_equiv(term *t1, term *t2)
 /*@ With term1 term2
       Require store_term(t1, term1) *
               store_term(t2, term2)
-      Ensure (__return == 1 && term_alpha_eq(term1, term2) || __return == 0 && !term_alpha_eq(term1, term2))
-       && t1 == t1@pre && t2 == t2@pre
-       && store_term(t1, term1) * store_term(t2, term2)
+      Ensure __return == term_alpha_eqn(term1, term2) && t1 == t1@pre && t2 == t2@pre
+   && store_term(t1, term1) * store_term(t2, term2)
 */
 {
   if (t1 == (void *)0 || t2 == (void *)0) return 0;
@@ -122,51 +121,18 @@ bool alpha_equiv(term *t1, term *t2)
       if (strcmp(t1->content.Quant.var, t2->content.Quant.var) == 0) {
         return alpha_equiv(t1->content.Quant.body, t2->content.Quant.body);
       } else {
-        /*@ 
-            exists y1 z1 qt1 qv1 qterm1 y2 z2 qt2 qv2 qterm2,
-              t1 != 0 && t2 != 0 &&
-              term1 == TermQuant(qt1, qv1, qterm1) &&
-              term2 == TermQuant(qt2, qv2, qterm2) &&
-              data_at(&(t1 -> type), termtypeID(term1)) *
-              data_at(&(t2 -> type), termtypeID(term2)) *
-              data_at(&(t1 -> content.Quant.type), qtID(qt1)) *
-              data_at(&(t2 -> content.Quant.type), qtID(qt2)) *
-              data_at(&(t1 -> content.Quant.var), y1) *
-              data_at(&(t2 -> content.Quant.var), y2) *
-              data_at(&(t1 -> content.Quant.body), z1) *
-              data_at(&(t2 -> content.Quant.body), z2) *
-              store_string(y1, qv1) * store_term(z1, qterm1) *
-              store_string(y2, qv2) * store_term(z2, qterm2)
+        /*@ exists qv1 qv2,
+            store_string(t1 -> content.Quant.var, qv1) *
+            store_string(t2 -> content.Quant.var, qv2) 
             which implies
-              store_term(t1, term1) * store_term(t2, term2)
+            t1 -> content.Quant.var != 0 &&
+            t2 -> content.Quant.var != 0 &&
+            store_string(t1 -> content.Quant.var, qv1) *
+            store_string(t2 -> content.Quant.var, qv2) 
         */
-        char *new_var = fresh(t1, t2);
-        /*@ 
-            termtypeID(term1) == 3 &&
-            termtypeID(term1) == termtypeID(term2) &&
-            store_term(t1, term1) * store_term(t2, term2)
-            which implies
-            exists y1 z1 qt1 qv1 qterm1 y2 z2 qt2 qv2 qterm2,
-              t1 != 0 && t2 != 0 &&
-              term1 == TermQuant(qt1, qv1, qterm1) &&
-              term2 == TermQuant(qt2, qv2, qterm2) &&
-              data_at(&(t1 -> type), termtypeID(term1)) *
-              data_at(&(t2 -> type), termtypeID(term2)) *
-              data_at(&(t1 -> content.Quant.type), qtID(qt1)) *
-              data_at(&(t2 -> content.Quant.type), qtID(qt2)) *
-              data_at(&(t1 -> content.Quant.var), y1) *
-              data_at(&(t2 -> content.Quant.var), y2) *
-              data_at(&(t1 -> content.Quant.body), z1) *
-              data_at(&(t2 -> content.Quant.body), z2) *
-              store_string(y1, qv1) * store_term(z1, qterm1) *
-              store_string(y2, qv2) * store_term(z2, qterm2)
-        */
-        term *new_t1 = subst_var(new_var, t1->content.Quant.var, copy_term(t1->content.Quant.body));
-        term *new_t2 = subst_var(new_var, t2->content.Quant.var, copy_term(t2->content.Quant.body));
-        bool result = alpha_equiv(new_t1, new_t2);
-        free_term(new_t1);
-        free_term(new_t2);
-        free_str(new_var);
+        term *t21 = subst_var(t1->content.Quant.var, t2->content.Quant.var, copy_term(t2->content.Quant.body));
+        bool result = alpha_equiv(t1->content.Quant.body, t21);
+        free_term(t21);
         return result;
       }
     }
