qcp/ast/VC/alpha_equiv_proof_manual.v
@@ -22,7 +22,7 @@ From SimpleC.EE Require Import sll_tmpl.
 Local Open Scope sac.
 
 Lemma proof_of_alpha_equiv_entail_wit_1 : alpha_equiv_entail_wit_1.
-Proof.
+Proof. 
   pre_process.
   unfold termtypeID in *.
   destruct term1; lia.
@@ -31,226 +31,205 @@ Qed.
 Lemma proof_of_alpha_equiv_return_wit_1_1 : alpha_equiv_return_wit_1_1.
 Proof.
   pre_process.
-  rewrite <- derivable1_orp_intros1.
+  unfold list_Z_cmp in H0.
+  destruct (list_Z_eqb str1 str2) eqn:Heq; [ contradiction | ].
+  unfold store_term, term_alpha_eqn, term_alpha_eq.
   rewrite H3, H4.
-  unfold store_term.
   Exists y z.
   entailer!.
-  intros Hc.
-  inversion Hc.
-  pose proof list_Z_eq2eqb str1 str2 H13.
-  unfold list_Z_cmp in H0.
-  rewrite H14 in H0.
-  congruence.
+  rewrite Heq.
+  reflexivity.
 Qed.
 
 Lemma proof_of_alpha_equiv_return_wit_1_2 : alpha_equiv_return_wit_1_2.
 Proof.
   pre_process.
-  rewrite <- derivable1_orp_intros2.
+  rewrite H in H0.
+  unfold list_Z_cmp in H0.
+  destruct (list_Z_eqb str1 str2) eqn:Heq; [ | discriminate ].
+  unfold store_term, term_alpha_eqn, term_alpha_eq.
   rewrite H3, H4.
-  unfold store_term.
   Exists y z.
   entailer!.
-  apply AlphaVar.
-  unfold list_Z_cmp in H0.
-  rewrite H in H0.
-  destruct (list_Z_eqb str1 str2) eqn:Heq; [ | congruence].
-  apply (list_Z_eqb2eq str1 str2 Heq).
+  rewrite Heq.
+  reflexivity.
 Qed.
 
 Lemma proof_of_alpha_equiv_return_wit_2 : alpha_equiv_return_wit_2.
 Proof.
   pre_process.
-  rewrite <- derivable1_orp_intros1.
-  rewrite H3, H2.
-  unfold store_term.
+  unfold store_term, term_alpha_eqn, term_alpha_eq.
+  rewrite H2, H3.
   entailer!.
-  intros Hc; inversion Hc.
-  congruence.
-Qed.  
+  destruct (ctID typ1 =? ctID typ2)%Z eqn:E.
+  + apply Z.eqb_eq in E.
+    contradiction.
+  + reflexivity.
+Qed.
 
 Lemma proof_of_alpha_equiv_return_wit_3_1 : alpha_equiv_return_wit_3_1.
-Proof.
+Proof. 
   pre_process.
-  rewrite <- derivable1_orp_intros1.
-  rewrite H4, H5.
   unfold store_term.
+  rewrite H4, H5.
   entailer!.
-  intros Hc; inversion Hc.
-  destruct H18; try congruence. 
+  unfold term_alpha_eqn, term_alpha_eq.
+  rewrite H1 at 1.
+  rewrite Z.eqb_refl.
+  destruct (con1 =? con2)%Z eqn:E.
+  + apply Z.eqb_eq in E.
+    contradiction.
+  + unfold negb.
+    rewrite H0.
+    reflexivity.
 Qed.
 
 Lemma proof_of_alpha_equiv_return_wit_3_2 : alpha_equiv_return_wit_3_2.
 Proof.
   pre_process.
-  rewrite <- derivable1_orp_intros2.
-  rewrite H4, H5.
   unfold store_term.
+  rewrite H4, H5.
   entailer!.
-  apply AlphaConst; [auto | right; auto].
+  unfold term_alpha_eqn, term_alpha_eq.
+  rewrite H1 at 1.
+  rewrite Z.eqb_refl.
+  destruct (con1 =? con2)%Z eqn:E.
+  + unfold negb.
+    rewrite H0.
+    reflexivity. 
+  + apply Z.eqb_neq in E.
+    contradiction.
 Qed.
 
 Lemma proof_of_alpha_equiv_return_wit_4 : alpha_equiv_return_wit_4.
 Proof.
   pre_process.
-  rewrite <- derivable1_orp_intros2.
-  rewrite H4, H3.
   unfold store_term.
+  rewrite H3, H4.
   entailer!.
-  apply AlphaConst; [auto | left; auto].
-Qed.
+  unfold term_alpha_eqn, term_alpha_eq.
+  rewrite H0 at 1.
+  rewrite Z.eqb_refl.
+  destruct (con1 =? con2)%Z eqn:E.
+  + unfold negb.
+    destruct (ctID typ1 =? 0)%Z eqn:Eq; [ | reflexivity].
+    apply Z.eqb_eq in E, Eq.
+    contradiction.
+  + unfold negb.
+    apply Z.eqb_neq in E.
+    destruct (ctID typ1 =? 0)%Z eqn:Eq; [ | reflexivity].
+    apply Z.eqb_eq in Eq.
+    contradiction.
+Qed.  
 
 Lemma proof_of_alpha_equiv_return_wit_5_1 : alpha_equiv_return_wit_5_1.
 Proof.
   pre_process.
-  rewrite <- derivable1_orp_intros2.
-  rewrite H8, H7.
-  unfold store_term; fold store_term.
+  unfold store_term.
+  rewrite H5, H6.
+  fold store_term.
   Exists y1 z1 y2 z2.
   entailer!.
-  apply AlphaApply; try auto.
+  unfold term_alpha_eqn in *.
+  unfold term_alpha_eq.
+  fold term_alpha_eq.
+  destruct (term_alpha_eq rt1 rt2) eqn:Eqr; [ | contradiction].
+  destruct (term_alpha_eq lt1 lt2) eqn:Eql; [ | contradiction].
+  reflexivity.
 Qed.
 
 Lemma proof_of_alpha_equiv_return_wit_5_2 : alpha_equiv_return_wit_5_2.
 Proof.
   pre_process.
+  unfold store_term.
+  rewrite H5, H6.
+  fold store_term.
+  Exists y1 z1 y2 z2.
+  entailer!.
+  unfold term_alpha_eqn in *.
+  unfold term_alpha_eq.
+  fold term_alpha_eq.
+  destruct (term_alpha_eq lt1 lt2) eqn:Eql; [ | contradiction].
+  destruct (term_alpha_eq rt1 rt2) eqn:Eqr; [ | reflexivity].
+  congruence.
 Qed.
 
 Lemma proof_of_alpha_equiv_return_wit_5_3 : alpha_equiv_return_wit_5_3.
-Proof. 
-  pre_process.
-Qed.
-
-Lemma proof_of_alpha_equiv_return_wit_5_4 : alpha_equiv_return_wit_5_4.
 Proof.
   pre_process.
-  rewrite <- derivable1_orp_intros1.
-  rewrite H7, H8.
-  unfold store_term; fold store_term.
+  unfold store_term.
+  rewrite H3, H4.
+  fold store_term.
   Exists y1 z1 y2 z2.
   entailer!.
-  contradict H1.
-  inversion H1.
-  auto.
-Qed.
-
-Lemma proof_of_alpha_equiv_return_wit_5_5 : alpha_equiv_return_wit_5_5.
-Proof.
-  pre_process.
-Qed.
-
-Lemma proof_of_alpha_equiv_return_wit_5_6 : alpha_equiv_return_wit_5_6.
-Proof.
-  pre_process.
-  rewrite <- derivable1_orp_intros1.
-  rewrite H4, H5.
-  unfold store_term; fold store_term.
-  Exists y1 z1 y2 z2.
-  entailer!.
-  contradict H1.
-  inversion H1.
-  auto.
+  unfold term_alpha_eqn in *.
+  unfold term_alpha_eq.
+  fold term_alpha_eq.
+  destruct (term_alpha_eq lt1 lt2) eqn:Eql; [ | reflexivity].
+  congruence.
 Qed.
 
 Lemma proof_of_alpha_equiv_return_wit_6 : alpha_equiv_return_wit_6.
 Proof.
   pre_process.
-  rewrite <- derivable1_orp_intros1.
+  unfold store_term.
   rewrite H2, H3.
-  unfold store_term; fold store_term.
+  fold store_term.
   Exists y1 z1 y2 z2.
   entailer!.
-  contradict H.
-  inversion H.
-  auto.
+  unfold term_alpha_eqn in *.
+  unfold term_alpha_eq.
+  fold term_alpha_eq.
+  destruct (qtID qt1 =? qtID qt2)%Z eqn:Eq; [ | reflexivity].
+  apply Z.eqb_eq in Eq.
+  congruence.
 Qed.
 
-Lemma proof_of_alpha_equiv_return_wit_7_1 : alpha_equiv_return_wit_7_1.
+Lemma proof_of_alpha_equiv_return_wit_7 : alpha_equiv_return_wit_7.
 Proof.
   pre_process.
-  rewrite <- derivable1_orp_intros2.
-  rewrite H6, H7.
-  unfold store_term; fold store_term.
+  unfold store_term.
+  rewrite H5, H6.
+  fold store_term.
   Exists y1 z1 y2 z2.
   entailer!.
-  apply AlphaQuant; [auto | left; split; [ | auto]].
-  unfold list_Z_cmp in H2.
-  destruct (list_Z_eqb qv1 qv2) eqn:Heq; [reflexivity | congruence].
+  unfold term_alpha_eqn in *.
+  unfold term_alpha_eq.
+  fold term_alpha_eq.
+  rewrite H0 in H1. 
+  unfold list_Z_cmp in H1.
+  destruct (qtID qt1 =? qtID qt2)%Z eqn:Eq.
+  + destruct (list_Z_eqb qv1 qv2) eqn:vEq; [ | congruence].
+    pose proof list_Z_eqb2eq qv1 qv2 vEq as vvEq.
+    pose proof (term_subst_v_same_name qv1 qv2 qterm2 vvEq) as qtEq.
+    rewrite qtEq.
+    tauto.
+  + destruct (list_Z_eqb qv1 qv2) eqn:vEq; [ | congruence].
+    rewrite Z.eqb_neq in Eq.
+    congruence.
 Qed.
 
-Lemma proof_of_alpha_equiv_return_wit_7_2 : alpha_equiv_return_wit_7_2.
+Lemma proof_of_alpha_equiv_return_wit_8 : alpha_equiv_return_wit_8.
 Proof.
   pre_process.
-  rewrite <- derivable1_orp_intros1.
-  rewrite H6, H7.
-  unfold store_term; fold store_term.
+  unfold store_term.
+  rewrite H9, H10.
+  fold store_term.
   Exists y1 z1 y2 z2.
-  entailer!.
-  contradict H0.
-  rewrite H1 in H2.
-  unfold list_Z_cmp in H2.
-  destruct list_Z_eqb eqn:Heqn; [ | congruence].
-  pose proof list_Z_eqb2eq qv1 qv2 Heqn as Heq.
-  inversion H0.
-  destruct H24 as [[Ha Hb] | Hc].
+  entailer!.  
+  unfold term_alpha_eqn in *.
+  unfold term_alpha_eq.
+  fold term_alpha_eq.
+  destruct (qtID qt1 =? qtID qt2)%Z eqn:Eq.
   + auto.
-  + destruct Hc; rewrite Heq in H24; congruence.
-Qed. 
-
-Lemma proof_of_alpha_equiv_return_wit_8_1 : alpha_equiv_return_wit_8_1.
-Proof. 
-    pre_process.
-    rewrite H, H7, H8.
-    rewrite <- derivable1_orp_intros2.
-    unfold store_term; fold store_term.
-    Exists y1 z1 y2 z2.
-    entailer!.
-    apply AlphaQuant.
-    + rewrite H7 in H16; injection H16; intros.
-      rewrite H8 in H17; injection H17; intros.
-      rewrite H29, H32; exact H13.
-    + right.
-      split.
-      - unfold list_Z_cmp in H12.
-        destruct (list_Z_eqb qv1 qv2) eqn:Heqq; [congruence | ].
-        rewrite H7 in H16; rewrite H8 in H17.
-        inversion H16; inversion H17; auto.
-      - exists str.
-        rewrite <- H7, <- H8.
-        auto.
-Qed.
-
-Lemma proof_of_alpha_equiv_return_wit_8_2 : alpha_equiv_return_wit_8_2.
-Proof.
-  pre_process.
-  rewrite H, H7, H8.
-  rewrite <- derivable1_orp_intros1.
-  unfold store_term; fold store_term.
-  Exists y1 z1 y2 z2.
-  entailer!.
-  contradict H0.
-  inversion H0.
-  destruct H34 as [Ha|Hb].
-  + destruct Ha as [Hc Hd].
-    rewrite H7 in H16; rewrite H8 in H17.
-    inversion H16; inversion H17.
-    unfold list_Z_cmp in H12.
-    destruct (list_Z_eqb qv1 qv2) eqn:Heqq; [congruence | ].
-    rewrite H36, H39 in *; congruence.
-  + destruct Hb as [Ha [x [Hx1 [Hx2 Hx3]]]].
-    apply (alpha_equiv_quant_allvar qterm1_2 qterm2_2 qt1_2 qt2_2 qv1_2 qv2_2 str).
-    auto.
-    rewrite H7 in H9; auto.
-    rewrite H8 in H10; auto. 
-    auto.
+  + rewrite Z.eqb_neq in Eq.
+    congruence.
 Qed.
 
 Lemma proof_of_alpha_equiv_return_wit_9_1 : alpha_equiv_return_wit_9_1.
 Proof. 
   pre_process.
   rewrite H.
-  rewrite <- derivable1_orp_intros1.
   apply store_null_right.
 Qed.
 
@@ -258,18 +237,16 @@ Lemma proof_of_alpha_equiv_return_wit_9_2 : alpha_equiv_return_wit_9_2.
 Proof.
   pre_process.
   rewrite H.
-  rewrite <- derivable1_orp_intros1.
   apply store_null_left.
 Qed.
 
 Lemma proof_of_alpha_equiv_return_wit_10 : alpha_equiv_return_wit_10.
 Proof.
   pre_process.
-  rewrite <- derivable1_orp_intros1.
   entailer!.
   2: {
     destruct term1; destruct term2; simpl in H; try lia.
-    all: unfold not; intros; inversion H4.
+    all: unfold term_alpha_eqn, term_alpha_eq; reflexivity.
   }
   pose proof (store_term_fold_out t2_pre term2) H1.
   sep_apply H4.
@@ -278,47 +255,15 @@ Proof.
   entailer!.
 Qed.
 
-Lemma proof_of_alpha_equiv_partial_solve_wit_16_pure : alpha_equiv_partial_solve_wit_16_pure.
-Proof. 
-  pre_process.
-  unfold store_string, NULL.
-  Intros n1 n2 n3.
-  entailer!.
-Qed.
-
-Lemma proof_of_alpha_equiv_partial_solve_wit_18_pure : alpha_equiv_partial_solve_wit_18_pure.
-Proof.
-  pre_process.
-  unfold store_string, NULL.
-  Intros n1 n2 n3.
-  entailer!.
-Qed.
-
-Lemma proof_of_alpha_equiv_partial_solve_wit_24_pure : alpha_equiv_partial_solve_wit_24_pure.
-Proof. 
-  pre_process.
-  unfold store_string, NULL.
-  Intros n1 n2 n3.
-  entailer!.
-Qed. 
-
-Lemma proof_of_alpha_equiv_partial_solve_wit_25_pure : alpha_equiv_partial_solve_wit_25_pure.
-Proof. 
-  pre_process.
-  unfold store_string, NULL.
-  Intros n1 n2 n3.
-  entailer!.
-Qed. 
-
 Lemma proof_of_alpha_equiv_which_implies_wit_1 : alpha_equiv_which_implies_wit_1.
-Proof.
+Proof. 
   pre_process.
   sep_apply store_term_unfold.
   sep_apply store_term_unfold.
   unfold NULL.
   entailer!.
 Qed.
-
+   
 Lemma proof_of_alpha_equiv_which_implies_wit_2 : alpha_equiv_which_implies_wit_2.
 Proof. 
   pre_process.
@@ -332,10 +277,10 @@ Proof.
   + rewrite <- H2; auto.
   + auto.
   + auto.
-Qed. 
+Qed.  
 
 Lemma proof_of_alpha_equiv_which_implies_wit_3 : alpha_equiv_which_implies_wit_3.
-Proof.
+Proof. 
   pre_process. 
   sep_apply store_term'_Const; unfold NULL.
   Intros ty1 c1.
@@ -347,10 +292,10 @@ Proof.
   + rewrite <- H2; auto.
   + auto.
   + auto.
-Qed.
+Qed. 
 
 Lemma proof_of_alpha_equiv_which_implies_wit_4 : alpha_equiv_which_implies_wit_4.
-Proof.
+Proof. 
   pre_process.
   sep_apply store_term'_Apply; unfold NULL.
   Intros ltt1 rtt1 yy1 zz1.
@@ -363,10 +308,10 @@ Proof.
   + rewrite <- H2; auto.
   + auto.
   + auto.
-Qed.
+Qed. 
 
 Lemma proof_of_alpha_equiv_which_implies_wit_5 : alpha_equiv_which_implies_wit_5.
-Proof. 
+Proof.  
   pre_process.
   sep_apply store_term'_Quant; unfold NULL.
   Intros qtt1 qvv1 bb1 yy1 zz1.
@@ -380,29 +325,14 @@ Proof.
   + rewrite <- H2; auto.
   + auto.
   + auto.
-Qed.
-
-Lemma proof_of_alpha_equiv_which_implies_wit_6 : alpha_equiv_which_implies_wit_6.
-Proof.
-  pre_process.
-  rewrite H1, H2.
-  unfold store_term; fold store_term.
-  Exists y1 z1 y2 z2.
-  entailer!.
-Qed.
-
-Lemma proof_of_alpha_equiv_which_implies_wit_7 : alpha_equiv_which_implies_wit_7.
-Proof.
-  pre_process.
-  rewrite H in H0.
-  unfold termtypeID in H, H0.
-  destruct term1; try discriminate.
-  destruct term2; try discriminate.
-  unfold store_term; fold store_term.
-  Intros yy1 zz1 yy2 zz2.
-  Exists zz2 zz1 yy2 yy1.
-  Exists qtype0 qvar0 term2.
-  Exists qtype qvar term1.
-  entailer!.
 Qed. 
 
+Lemma proof_of_alpha_equiv_which_implies_wit_6 : alpha_equiv_which_implies_wit_6.
+Proof. 
+  pre_process.
+  unfold store_string.
+  unfold NULL.
+  Intros x n.
+  Exists x n.
+  entailer!.
+Qed. 
